move Mapping type and related definitions from smcapi.s to pagedb.s
This kludge allows ptebits.i to avoid including smcapi.s and all its
new dependencies, which in turn appears to fix an instability problem
with bitvector proofs.

verified/pagedb.s.dfy
@@ -314,3 +314,40 @@ predicate validAddrspacePage(d: PageDb, a: int)
 {
     wellFormedPageDb(d) && isAddrspace(d, a)
 }
+
+//=============================================================================
+// Mapping
+//=============================================================================
+datatype Mapping = Mapping(l1index: word, l2index: word, perm: Perm)
+datatype Perm = Perm(r: bool, w: bool, x: bool)
+
+predicate validMapping(m:Mapping,d:PageDb,a:PageNr)
+{
+    reveal_validPageDb();
+    validPageDb(d) && isAddrspace(d,a) && validAddrspace(d,a) 
+    && validPageNr(m.l1index) && 0 <= m.l1index < NR_L1PTES()
+    && validPageNr(m.l2index) && 0 <= m.l2index < NR_L2PTES()
+    && (var addrspace := d[a].entry;
+        addrspace.state == InitState &&
+        (var l1 := d[addrspace.l1ptnr].entry;
+        l1.l1pt[m.l1index].Just?))
+}
+
+function l1indexFromMapping(arg:word) : word
+    { RightShift(arg,20) }
+
+function l2indexFromMapping(arg:word) : word
+    { BitwiseAnd(RightShift(arg,12),0xff) }
+
+function permFromMapping(arg:word) : Perm
+{
+    Perm(BitwiseAnd(arg,KOM_MAPPING_R()) != 0,
+        BitwiseAnd(arg,KOM_MAPPING_W()) != 0,
+        BitwiseAnd(arg,KOM_MAPPING_X()) != 0)
+}
+
+function {:opaque} wordToMapping(arg:word) : Mapping
+{
+    Mapping(l1indexFromMapping(arg),l2indexFromMapping(arg),
+        permFromMapping(arg))
+}
